Add synthesizable unsigned multiplier (#324)

cava/Cava/Monad/NetlistGeneration.v
@@ -200,6 +200,15 @@ Definition unsignedAddNet {m n : nat}
   let smashedSum := Vector.map (fun i => IndexConst sum i) (vseq 0 (1 + (max m n))) in
   ret smashedSum.
 
+Definition unsignedMultNet {m n : nat}
+                          (a : Vector.t (Signal Bit) m)
+                          (b : Vector.t (Signal Bit) n) :
+                          state CavaState (Vector.t (Signal Bit) (m + n)) :=
+  product <- newVector Bit (m + n) ;;
+  addInstance (UnsignedMultiply (VecLit a) (VecLit b) product) ;;
+  let smashedMult := Vector.map (fun i => IndexConst product i) (vseq 0 (m + n)) in
+  ret smashedMult.
+
 Definition delayBitNet (i : Signal Bit) : state CavaState (Signal Bit) :=
   o <- newWire ;;
   addInstance (DelayBit i o) ;;
@@ -278,6 +287,7 @@ Instance CavaNet : Cava (state CavaState) (Signal _) :=
     indexBitConst sz := @indexConstNet Bit sz;
     slice k sz start len v h := @sliceNet k sz start len v h;
     unsignedAdd m n := @unsignedAddNet m n;
+    unsignedMult m n := @unsignedMultNet m n;
     greaterThanOrEqual m n := @greaterThanOrEqualNet m n;
     instantiate := instantiateNet;
 }.
